src/riscv/Platform/MetricMaterializeRiscvProgram.v
@@ -1,0 +1,42 @@
+Require Import Coq.ZArith.ZArith.
+Require Import coqutil.Word.Interface coqutil.Word.Bitwidth.
+Require Import riscv.Utility.Monads.
+Require Import riscv.Utility.FreeMonad.
+Require Import riscv.Spec.Machine.
+Require Import riscv.Platform.MetricLogging.
+Require Import riscv.Platform.MaterializeRiscvProgram.
+
+Section Riscv.
+  Import free.
+
+  Context {width: Z} {BW: Bitwidth width} {word: word width}.
+
+  Definition action : Type := (MetricLog -> MetricLog) * riscv_primitive.
+  Definition result (a : action) := primitive_result (snd a).
+
+  Global Instance MetricMaterialize: RiscvProgram (free action result) word := {|
+    getRegister a := act (id, GetRegister a) ret;
+    setRegister a b := act (id, SetRegister a b) ret;
+    loadByte a b := act (addMetricLoads 1, LoadByte a b) ret;
+    loadHalf a b := act (addMetricLoads 1, LoadHalf a b) ret;
+    loadWord a b := act (addMetricLoads 1, LoadWord a b) ret;
+    loadDouble a b := act (addMetricLoads 1, LoadDouble a b) ret;
+    storeByte a b c := act (addMetricStores 1, StoreByte a b c) ret;
+    storeHalf a b c := act (addMetricStores 1, StoreHalf a b c) ret;
+    storeWord a b c := act (addMetricStores 1, StoreWord a b c) ret;
+    storeDouble a b c := act (addMetricStores 1, StoreDouble a b c) ret;
+    makeReservation a := act (id, MakeReservation a) ret;
+    clearReservation a := act (id, ClearReservation a) ret;
+    checkReservation a := act (id, CheckReservation a) ret;
+    getCSRField f := act (id, GetCSRField f) ret;
+    setCSRField f v := act (id, SetCSRField f v) ret;
+    getPrivMode := act (id, GetPrivMode) ret;
+    setPrivMode m := act (id, SetPrivMode m) ret;
+    fence a b := act (id, Fence a b) ret;
+    getPC := act (id, GetPC) ret;
+    setPC a := act (addMetricJumps 1, SetPC a) ret;
+    endCycleNormal := act (addMetricInstructions 1, EndCycleNormal) ret;
+    endCycleEarly A := act (addMetricInstructions 1, EndCycleEarly A) ret;
+  |}.
+
+End Riscv.
